feat(TestModels): Extendable Data now returns Resource Name
From PR #137, resolves:
- https://github.com/awslabs/polymorph/pull/137#discussion_r1102273747
- https://github.com/awslabs/polymorph/pull/137#discussion_r1102264195
- https://github.com/awslabs/polymorph/pull/137#discussion_r1102265063

TestModels/Extendable/runtimes/net/Extern/NativeResource.cs
@@ -40,6 +40,7 @@ namespace Simple.Extendable.Resources
     public static NativeResource NativeFactory()
     {
       ExtendableResource_Compile.ExtendableResource _nw2 = new ExtendableResource_Compile.ExtendableResource();
+      _nw2.__ctor();
       IExtendableResource dafnyResource =
         TypeConversion.FromDafny_N6_simple__N10_extendable__N9_resources__S27_ExtendableResourceReference(_nw2);
       return new NativeResource(dafnyResource);
