TestModels/Extendable/src/Index.dfy
@@ -14,27 +14,20 @@ module
   {SimpleExtendableResourcesConfig()}
 
   method SimpleExtendableResources(
+    // SimpleExtendableResourcesConfig is an empty structure,
+    // so the `config` parameter is ignored,
+    // but smithy-dafny generates it,
+    // so the implementation MUST have it.
     config: SimpleExtendableResourcesConfig
   ) returns (
     res: Result<SimpleExtendableResourcesClient, Error>
   )
   {
-    // SimpleExtendableResourcesConfig is an empty structure,
-    // so the `config` parameter is ignored,
-    // but smithy-dafny generates it,
-    // so the implementation MUST have it.
     var internalConfig := Operations.Config();
-
-    if Operations.ValidInternalConfig?(internalConfig) {
-      var client := new SimpleExtendableResourcesClient(
-        config := internalConfig
-      );
-      return Success(client);
-    } else {
-      return Failure(Types.SimpleExtendableResourcesException(
-        message := "Invalid Internal Config. Should be impossible.")
-      );
-    }
+    var client := new SimpleExtendableResourcesClient(
+      config := internalConfig
+    );
+    return Success(client);
   }
 
   class SimpleExtendableResourcesClient...
